added code for extfzl/extfsl (not very useful since bitfields are limited to 32 bits)

common/Values.v
@@ -802,7 +802,7 @@ Definition extfzl stop start v :=
     let stop' := Z.add stop Z.one in
     match v with
     | Vlong w =>
-      Vlong (Int64.shru (Int64.shl w (Int64.repr (Z.sub Int64.zwordsize stop'))) (Int64.repr (Z.sub Int64.zwordsize (Z.sub stop' start))))
+      Vlong (Int64.shru' (Int64.shl' w (Int.repr (Z.sub Int64.zwordsize stop'))) (Int.repr (Z.sub Int64.zwordsize (Z.sub stop' start))))
     | _ => Vundef
     end
   else Vundef.
@@ -816,7 +816,7 @@ Definition extfsl stop start v :=
     let stop' := Z.add stop Z.one in
     match v with
     | Vlong w =>
-      Vlong (Int64.shr (Int64.shl w (Int64.repr (Z.sub Int64.zwordsize stop'))) (Int64.repr (Z.sub Int64.zwordsize (Z.sub stop' start))))
+      Vlong (Int64.shr' (Int64.shl' w (Int.repr (Z.sub Int64.zwordsize stop'))) (Int.repr (Z.sub Int64.zwordsize (Z.sub stop' start))))
     | _ => Vundef
     end
   else Vundef.
